---
title: ""
output: pdf_document
---

# Ejercicio 2

Considere el modelo de regresion
$$
y_i=\beta_0+\beta_1 x_i+\beta_2\left(3 x_i^2-2\right)+\xi_i \quad i=1,2,3
$$
donde
$$
x_1=-1, x_2=0, x_3=1
$$
I)
Matriz de dise√±o
$$
X=\left(\begin{array}{rrr}
1 & -1 & 1 \\
1 & 0 & -2 \\
1 & 1 & 1
\end{array}\right) \text { pues } \begin{aligned}
& 3 x_1^2-2=1 \\
& 3 x_2^2-2=-2 \\
& 3 x_3^2-2=1
\end{aligned}
$$

Asi
$$
\begin{aligned}
& X^t X=\left(\begin{array}{ccc}
1 & 1 & 1 \\
-1 & 0 & 1 \\
1 & -2 & 1
\end{array}\right)\left(\begin{array}{ccc}
1 & -1 & 1 \\
1 & 0 & -2 \\
1 & 1 & 1
\end{array}\right)=\left(\begin{array}{lll}
3 & 0 & 0 \\
0 & 2 & 0 \\
0 & 0 & 6
\end{array}\right) \\
& y \\
& \left(X^t X\right)^{-1}=\left(\begin{array}{ccc}
1 / 3 & 0 & 0 \\
0 & 1 / 2 & 0 \\
0 & 0 & 1 / 6
\end{array}\right)
\end{aligned}
$$
II)

$$
\hat{\beta}=(X^t X)^{-1} X^t y
$$
asi:
$$
\begin{aligned}
& \hat{\beta}=\left(\begin{array}{ccc}
1 / 3 & 0 & 0 \\
0 & 1 / 2 & 0 \\
0 & 0 & 1 / 6
\end{array}\right)\left(\begin{array}{ccc}
1 & 1 & 1 \\
-1 & 0 & 1 \\
1 & -2 & 1
\end{array}\right)\left(\begin{array}{l}
y_1 \\
y_2 \\
y_3
\end{array}\right)=\left(\begin{array}{ccc}
1 / 3 & 1 / 3 & 1 / 3 \\
-1 / 2 & 0 & 1 / 2 \\
1 / 6 & -1 / 3 & 1 / 6
\end{array}\right)\left(\begin{array}{l}
y_1 \\
y_2 \\
y_3
\end{array}\right) \\
& \hat{\beta}=\left(\begin{array}{l}
\frac{1}{3}\left(y_1+y_2+y_3\right) \\
\frac{1}{2}\left(y_3-y_1\right) \\
\frac{1}{6}\left(y_1-2 y_2+y_3\right)
\end{array}\right)
\end{aligned}
$$

Por lo tanto
$$
\hat{\beta}_0=\frac{1}{3}\left(y_1+y_2+y_3\right) \quad \hat{\beta}_1=\frac{1}{2}\left(y_3-y_1\right) \quad \hat{\beta}_2=\frac{1}{6}\left(y_1-2 y_2+y_3\right)
$$
III)
Obtenemos los estimadores del modelo reducido:
$$
y_i=\beta_0^*+\beta_1^* x_i+\xi_i^* \quad i=1,2,3
$$

Obtenemos
$$
\begin{aligned}
& \left(X^t X\right)^{-1}=\left(\begin{array}{cc}
1 / 3 & 0 \\
0 & 1 / 2
\end{array}\right) \\
&
\end{aligned}
$$
$$\begin{aligned} & \rightarrow \hat{\beta}^*=\left(\begin{array}{cc}1 / 3 & 0 \\ 0 & 1 / 2\end{array}\right)\left(\begin{array}{ccc}1 & 1 & 1 \\ -1 & 0 & 1\end{array}\right)\left(\begin{array}{l}y_1 \\ y_2 \\ y_3\end{array}\right)=\left(\begin{array}{ccc}1 / 3 & 1 / 3 & 1 / 3 \\ -1 / 2 & 0 & 1 / 2\end{array}\right)\left(\begin{array}{l}y_1 \\ y_2 \\ y_3\end{array}\right) \\ & \hat{\beta}^*=\binom{\frac{1}{3}\left(y_1+y_2+y_3\right)}{\frac{1}{2}\left(y_3-y_1\right)} \\ & \text { Asi } \hat{\beta}_0^*=\frac{1}{3}\left(y_1+y_2+y_3\right) \text { y } \hat{\beta}_1^*=\frac{1}{2}\left(y_3-y_1\right) \\ \therefore \hat{\beta}_0^*=\hat{\beta}_0 \text { y } \hat{\beta}_1^*=\hat{\beta}_1 \\ & \end{aligned}$$